backends/lean/Aeneas/Array.lean
@@ -1,0 +1,91 @@
+import Aeneas.List
+import Aeneas.SimpIfs
+
+namespace Array
+
+attribute [-simp] List.getElem!_eq_getElem?_getD
+
+def setSlice! {α} (a : Array α) (i : ℕ) (s : List α) : Array α :=
+  ⟨ a.toList.setSlice! i s⟩
+
+@[local simp]
+theorem getElem!_eq_toList_getElem! {α} [Inhabited α] (s : Array α) (i : ℕ) :
+  s[i]! = s.toList[i]! := by
+  cases s; simp
+
+@[local simp]
+theorem getElem_eq_toList_getElem {α} [Inhabited α] (s : Array α) (i : ℕ) (hi : i < s.size) :
+  s[i] = s.toList[i] := by
+  cases s; simp
+
+@[simp, simp_lists_simps]
+theorem getElem!_default [Inhabited α] (ls : Array α) (i : ℕ)
+  (h : ls.size ≤ i) : ls[i]! = default := by
+  simp only [getElem!_eq_toList_getElem!]; simp_lists
+
+@[simp, simp_lists_simps, scalar_tac_simps]
+theorem setSlice!_length {α} (s : Array α) (i : ℕ) (s' : List α) :
+  (s.setSlice! i s').size = s.size := by
+  simp only [setSlice!, List.size_toArray, List.setSlice!_length, length_toList]
+
+theorem setSlice!_getElem!_prefix {α} [Inhabited α]
+  (s : Array α) (s' : List α) (i j : ℕ) (h : j < i) :
+  (s.setSlice! i s')[j]! = s[j]! := by
+  simp only [setSlice!, getElem!_eq_toList_getElem!]
+  simp_lists
+
+@[simp_lists_simps]
+theorem setSlice!_getElem!_middle {α} [Inhabited α]
+  (s : Array α) (s' : List α) (i j : ℕ) (h : i ≤ j ∧ j - i < s'.length ∧ j < s.size) :
+  (s.setSlice! i s')[j]! = s'[j - i]! := by
+  simp only [setSlice!, getElem!_eq_toList_getElem!]
+  simp_lists
+
+theorem setSlice!_getElem!_suffix {α} [Inhabited α]
+  (s : Array α) (s' : List α) (i j : ℕ) (h : i + s'.length ≤ j) :
+  (s.setSlice! i s')[j]! = s[j]! := by
+  simp only [setSlice!, getElem!_eq_toList_getElem!]
+  simp_lists
+
+@[simp_lists_simps]
+theorem setSlice!_getElem!_same {α} [Inhabited α] (s : Array α) (s' : List α) (i j : ℕ)
+  (h : j < i ∨ i + s'.length ≤ j) :
+  (s.setSlice! i s')[j]! = s[j]! := by
+  cases h <;> simp_lists [setSlice!_getElem!_prefix, setSlice!_getElem!_suffix]
+
+@[simp_lists_simps]
+def Inhabited_getElem_eq_getElem! {α} [Inhabited α] (l : Array α) (i : ℕ) (hi : i < l.size) :
+  l[i] = l[i]! := by
+  simp only [getElem_eq_toList_getElem, List.Inhabited_getElem_eq_getElem!,
+    getElem!_eq_toList_getElem!]
+
+@[simp_lists_simps]
+theorem set_eq_set! (a : Array α) (i : ℕ) (x : α) (hi : i < a.size) :
+  a.set i x hi = a.set! i x := by
+  simp only [Array.set, Array.set!, Array.setIfInBounds, hi, ↓reduceDIte]
+
+@[simp, simp_lists_simps]
+theorem getElem!_set! {α : Type u}
+  [Inhabited α] {i j : ℕ} {x : α} {xs : Array α}
+  (hi : i < xs.size ∧ j = i) :
+  (xs.set! i x)[j]! = x := by
+  simp only [set!_eq_setIfInBounds, getElem!_eq_toList_getElem!, toList_setIfInBounds]
+  simp_lists
+
+@[simp, simp_lists_simps]
+theorem getElem!_set!_ne {α : Type u}
+  [Inhabited α] {i j : ℕ} {x : α} {xs : Array α}
+  (h : i ≠ j) :
+  (xs.set! i x)[j]! = xs[j]! := by
+  simp only [set!_eq_setIfInBounds, getElem!_eq_toList_getElem!, toList_setIfInBounds]
+  simp_lists
+
+@[simp, simp_lists_simps]
+theorem getElem!_replicate {α : Type u} [Inhabited α] {i n : ℕ} {a : α} (h : i < n) :
+  (Array.replicate n a)[i]! = a := by
+  unfold getElem! Array.instGetElem?NatLtSize Array.get!Internal
+  simp only [Array.getD_eq_getD_getElem?, Array.getElem?_replicate]
+  simp_ifs
+  simp only [Option.getD_some]
+
+end Array
