backends/lean/Aeneas/Bvify/Bvify.lean
@@ -25,6 +25,7 @@ attribute [bvify_simps]
   Int.reduceLT Int.reduceLE Int.reduceGT Int.reduceGE Int.reduceEq Int.reduceNe Int.reduceBEq Int.reduceBNe
   Int.reducePow Int.reduceAdd Int.reduceSub Int.reduceMul Int.reduceDiv Int.reduceMod
   Int.reduceNegSucc Int.reduceNeg Int.reduceToNat
+  BitVec.reduceMul BitVec.reduceAdd BitVec.reduceSub BitVec.reduceMod BitVec.reduceDiv
 
 @[simp, bvify_simps] theorem U8.UScalar_bv (x : U8) : UScalar.bv x = x.bv := by simp
 @[simp, bvify_simps] theorem U16.UScalar_bv (x : U16) : UScalar.bv x = x.bv := by simp
