backends/lean/Aeneas/Byte.lean
@@ -1,0 +1,6 @@
+import Lean
+
+abbrev Byte := BitVec 8
+abbrev Byte.ofNat := BitVec.ofNat 8
+abbrev Byte.val (b : Byte) := @BitVec.toNat 8 b
+abbrev Byte.testBit (b : Byte) := Nat.testBit b.toNat
