backends/lean/Aeneas/SimpLists.lean
@@ -1,1 +1,2 @@
 import Aeneas.SimpLists.SimpLists
+import Aeneas.SimpLists.Tests
