backends/lean/Aeneas/SimpLists/SimpLists.lean
@@ -1,6 +1,5 @@
 import Aeneas.SimpLists.Init
 import Aeneas.ScalarTac.CondSimpTac
-import Aeneas.List.List
 
 /-!
 # `simp_lists` tactic
@@ -13,7 +12,9 @@ namespace Aeneas.SimpLists
 
 open Lean Lean.Meta Lean.Parser.Tactic Lean.Elab.Tactic
 
-attribute [simp_lists_simps] add_tsub_cancel_right add_tsub_cancel_left
+attribute [simp_lists_simps]
+  add_tsub_cancel_right add_tsub_cancel_left Bool.false_or Bool.or_false
+  implies_true
 
 structure Args where
   declsToUnfold : Array Name := #[]
@@ -86,29 +87,5 @@ elab stx:simp_lists : tactic =>
   withMainContext do
   let (args, loc) ← parseSimpLists stx
   simpListsTac args loc
-
-example [Inhabited α] (l : List α) (x : α) (i j : Nat) (hj : i ≠ j) : (l.set j x)[i]! = l[i]! := by
-  simp_lists
-
-example [Inhabited α] (l : List α) (x : α) (i : Nat) (hi : i < l.length) : (l.set i x)[i]! = x := by
-  simp_lists
-
-/-- We use this lemma to "normalize" successive calls to `List.set` -/
-@[simp_lists_simps]
-theorem List.set_comm_lt (a b : α) (n m : Nat) (l : List α) (h : n < m) :
-  (l.set m a).set n b = (l.set n b).set m a := by
-  rw [List.set_comm]
-  omega
-
-example [Inhabited α] (l : List α) (x y : α) (i j : Nat) (hj : i < j) : (l.set i x).set j y = (l.set j y).set i x := by
-  simp_lists
-
-example (CList : Type) (l : CList) (get : CList → Nat → Bool) (set : CList → Nat → Bool → CList)
-  (h : ∀ i j l x, i ≠ j → get (set l i x) j = get l j) (i j : Nat) (hi : i < j) : get (set l i x) j = get l j := by
-  simp_lists [h]
-
-example (CList : Type) (l : CList) (get : CList → Nat → Bool) (set : CList → Nat → Bool → CList)
-  (h : ∀ i j l x, i ≠ j → get (set l i x) j = get l j) (i j : Nat) (hi : i < j) : get (set l i x) j = get l j := by
-  simp_lists [*]
 
 end Aeneas.SimpLists
