backends/lean/Aeneas/Vector.lean
@@ -1,0 +1,113 @@
+import Aeneas.Array
+
+namespace Vector
+
+attribute [-simp] List.getElem!_eq_getElem?_getD
+attribute [local simp] Array.getElem!_eq_toList_getElem! Array.getElem_eq_toList_getElem
+attribute [scalar_tac self.toArray] Vector.size_toArray
+
+@[scalar_tac xs.toList]
+theorem toList_length {α : Type u} {n : ℕ} (xs : Vector α n) :
+  xs.toList.length = n := by
+  simp only [Array.length_toList, size_toArray]
+
+def setSlice! {α} {n} (a : Vector α n) (i : ℕ) (s : List α) : Vector α n :=
+  ⟨ a.toArray.setSlice! i s, by simp only [Array.setSlice!_length, size_toArray] ⟩
+
+attribute [local simp] List.Inhabited_getElem_eq_getElem! Array.Inhabited_getElem_eq_getElem!
+
+@[local simp]
+theorem getElem!_eq_toArray_getElem! {α} {n} [Inhabited α] (s : Vector α n) (i : ℕ) :
+  s[i]! = s.toArray[i]! := by
+  cases s; simp
+  unfold instGetElem?OfGetElemOfDecidable decidableGetElem?
+  simp; split <;> simp_all only [Option.ite_none_right_eq_some, Option.some.injEq, ite_eq_right_iff]
+  simp_all
+  rfl
+
+@[simp, simp_lists_simps]
+theorem getElem!_default [Inhabited α] (ls : Vector α n) (i : ℕ)
+  (h : n ≤ i) : ls[i]! = default := by
+  have : ls.toArray.size ≤ i := by scalar_tac
+  simp only [getElem!_eq_toArray_getElem!]; simp_lists
+
+@[local simp]
+theorem getElem_eq_toArray_getElem {α} {n} [Inhabited α] (s : Vector α n) (i : ℕ) (hi : i < n) :
+  s[i] = getElem s.toArray i (by have := s.size_toArray; omega) := by
+  cases s; simp
+
+@[simp, simp_lists_simps, scalar_tac_simps]
+theorem setSlice!_length {α} {n} (s : Vector α n) (i : ℕ) (s' : List α) :
+  (s.setSlice! i s').size = n := by
+  simp only [size_toArray]
+
+theorem setSlice!_getElem!_prefix {α} {n} [Inhabited α]
+  (s : Vector α n) (s' : List α) (i j : ℕ) (h : j < i) :
+  (s.setSlice! i s')[j]! = s[j]! := by
+  simp only [getElem!_eq_toArray_getElem!, setSlice!]
+  simp_lists
+
+@[simp_lists_simps]
+theorem setSlice!_getElem!_middle {α} {n} [Inhabited α]
+  (s : Vector α n) (s' : List α) (i j : ℕ) (h : i ≤ j ∧ j - i < s'.length ∧ j < s.size) :
+  (s.setSlice! i s')[j]! = s'[j - i]! := by
+  simp only [setSlice!, getElem!_eq_toArray_getElem!]
+  simp_lists
+
+theorem setSlice!_getElem!_suffix {α} {n} [Inhabited α]
+  (s : Vector α n) (s' : List α) (i j : ℕ) (h : i + s'.length ≤ j) :
+  (s.setSlice! i s')[j]! = s[j]! := by
+  simp only [setSlice!, getElem!_eq_toArray_getElem!]
+  simp_lists
+
+@[simp_lists_simps]
+theorem setSlice!_getElem!_same {α} {n} [Inhabited α] (s : Vector α n) (s' : List α) (i j : ℕ)
+  (h : j < i ∨ i + s'.length ≤ j) :
+  (s.setSlice! i s')[j]! = s[j]! := by
+  cases h <;> simp_lists [setSlice!_getElem!_prefix, setSlice!_getElem!_suffix]
+
+@[simp_lists_simps]
+def Inhabited_getElem_eq_getElem! {α} {n} [Inhabited α] (l : Vector α n) (i : ℕ) (hi : i < n) :
+  l[i] = l[i]! := by
+  simp only [getElem_eq_toArray_getElem, Array.Inhabited_getElem_eq_getElem!,
+    getElem!_eq_toArray_getElem!]
+
+@[simp_lists_simps]
+theorem set_eq_set! (v : Vector α n) (i : ℕ) (x : α) (hi : i < n) :
+  v.set i x hi = v.set! i x := by
+  simp only [Vector.set, Array.set_eq_set!, Vector.set!]
+
+@[simp, simp_lists_simps]
+theorem getElem!_set! {α : Type u}
+  [Inhabited α] {n i j : ℕ} {x : α} {xs : Vector α n}
+  (hi : i < n ∧ j = i) :
+  (xs.set! i x)[j]! = x := by
+  have : i < xs.toArray.size := by scalar_tac
+  simp only [getElem!_eq_toArray_getElem!, toArray_set!, Array.set!_eq_setIfInBounds,
+    Array.getElem!_eq_toList_getElem!, Array.toList_setIfInBounds]
+  simp_lists
+
+@[simp, simp_lists_simps]
+theorem getElem!_set!_ne {α : Type u}
+  [Inhabited α] {n i j : ℕ} {x : α} {xs : Vector α n}
+  (h : i ≠ j) :
+  (xs.set! i x)[j]! = xs[j]! := by
+  simp
+  simp_lists
+
+@[simp, simp_lists_simps]
+theorem getElem!_replicate {α : Type u} [Inhabited α] {i n : ℕ} {a : α} (h : i < n) :
+ (Vector.replicate n a)[i]! = a := by
+ unfold getElem! instGetElem?OfGetElemOfDecidable Vector.instGetElemNatLt decidableGetElem? Vector.get
+ simp; simp_lists
+ split_ifs
+ simp
+
+
+@[simp, simp_lists_simps]
+theorem getElem!_cast {n m : ℕ} {α : Type u_1} [Inhabited α] (h: n = m) (v : Vector α n) (i : ℕ):
+  (Vector.cast h v)[i]! = v[i]! := by
+  simp only [getElem!_eq_toArray_getElem!, toArray_cast, Array.getElem!_eq_toList_getElem!]
+
+
+end Vector
